cont-passing interpreter without decreasing fuel too much

shift-reset/interpreter/interpreter.v
@@ -1,167 +1,189 @@
-From Stdlib Require Import String ZArith.
-From shift_reset.core Require Import syntax var venv.
+From Stdlib Require Import String ZArith Lia.
+From shift_reset.core Require Import syntax var env.
 From shift_reset.interpreter Require Import istate ierror imonad.
 
 Local Open Scope string_scope.
 Local Open Scope Z_scope.
 
-Definition interpret_expr1_aux (go : expr -> imonad val) (e : expr1) (v : val) : imonad val :=
-  let (b, e') := e in
-  match b with
-  | BAnon => go e'
-  | BVar x => imonad_local_env (VECons x v) (go e')
+Definition interpret_atom (a : atom) : imonad val :=
+  match a with
+  | AVal v => imonad_pure v
+  | AVar x => imonad_bind imonad_ask_env
+                (fun env => match env_lookup x env with
+                            | None => imonad_throw (NameError "")
+                            | Some v => imonad_pure v
+                            end)
   end.
 
-Definition interpret_expr2_aux (go : expr -> imonad val) (e : expr2) (v1 v2 : val) : imonad val :=
-  let (b, e') := e in
+Definition interpret_term1_aux (go : term -> imonad val) (t : term1) (v : val) : imonad val :=
+  let (b, t') := t in
   match b with
-  | BAnon => interpret_expr1_aux go e' v2
-  | BVar x => imonad_local_env (VECons x v1) (interpret_expr1_aux go e' v2)
+  | BAnon => go t'
+  | BVar x => imonad_local_env (ECons x v) (go t')
   end.
+
+Definition interpret_term2_aux (go : term -> imonad val) (t : term2) (v1 v2 : val) : imonad val :=
+  let (b, t') := t in
+  match b with
+  | BAnon => interpret_term1_aux go t' v2
+  | BVar x => imonad_local_env (ECons x v1) (interpret_term1_aux go t' v2)
+  end.
+
+Definition interpret_clo1_aux (go : term -> imonad val) (c : clo1) (v : val) : imonad val :=
+  let (t, env) := c in imonad_local_env (fun _ => env) (interpret_term1_aux go t v).
+
+Definition interpret_clo2_aux (go : term -> imonad val) (c : clo2) (v1 v2 : val) : imonad val :=
+  let (t, env) := c in imonad_local_env (fun _ => env) (interpret_term2_aux go t v1 v2).
+
+(*
+Definition interpret_kont_aux (go : kont -> term -> imonad val) (k : kont) (v : val) : imonad val :=
+  match k with
+  | KNil => imonad_pure v
+  | KCons c k' => interpret_clo1_aux (go k') c v
+  end.
+*)
 
 Definition interpret_let : imonad val -> (val -> imonad val) -> imonad val :=
   imonad_bind.
 
-Definition interpret_if (a e1 e2 : imonad val) :=
-  imonad_bind a
+Definition interpret_if (a : atom) (t1 t2 : imonad val) :=
+  imonad_bind (interpret_atom a)
     (fun v => match v with
-              | VBool b => if b then e1 else e2
+              | VBool b => if b then t1 else t2
               | _ => imonad_throw (TypeError "")
               end).
 
-Definition interpret_prim1 (p : prim1) (a : imonad val) : imonad val :=
-  imonad_bind a
+Definition interpret_prim1 (p : prim1) (a : atom) : imonad val :=
+  imonad_bind (interpret_atom a)
     (fun v => match p, v with
               | P1Neg, VInt i => imonad_pure (VInt (-i))
               | P1Not, VBool b => imonad_pure (VBool (negb b))
               | _, _ => imonad_throw (TypeError "")
               end).
 
-Definition interpret_prim2 (p : prim2) (a1 a2 : imonad val) : imonad val :=
+Definition interpret_prim2_aux (p : prim2) (a1 a2 : imonad val) : imonad val :=
   imonad_bind a1
     (fun v1 =>
        match p, v1 with
-       | P2Add, VInt i1 =>
-           imonad_bind a2
-             (fun v2 => match v2 with
-                        | VInt i2 => imonad_pure (VInt (i1 + i2))
-                        | _ => imonad_throw (TypeError "")
-                        end)
-       | P2Sub, VInt i1 =>
-           imonad_bind a2
-             (fun v2 => match v2 with
-                        | VInt i2 => imonad_pure (VInt (i1 - i2))
-                        | _ => imonad_throw (TypeError "")
-                        end)
-       | P2Mul, VInt i1 =>
-           imonad_bind a2
-             (fun v2 => match v2 with
-                        | VInt i2 => imonad_pure (VInt (i1 * i2))
-                        | _ => imonad_throw (TypeError "")
-                        end)
-       | P2Div, VInt i1 =>
-           imonad_bind a2
-             (fun v2 => match v2 with
-                        | VInt i2 => imonad_pure (VInt (i1 / i2))
-                        | _ => imonad_throw (TypeError "")
-                        end)
-       | P2Rem, VInt i1 =>
-           imonad_bind a2
-             (fun v2 => match v2 with
-                        | VInt i2 => imonad_pure (VInt (Z.rem i1 i2))
-                        | _ => imonad_throw (TypeError "")
-                        end)
-       | P2And, VBool b1 =>
-           imonad_bind a2
-             (fun v2 => match v2 with
-                        | VBool b2 => imonad_pure (VBool (b1 && b2))
-                        | _ => imonad_throw (TypeError "")
-                        end)
-       | P2Or, VBool b1 =>
-           imonad_bind a2
-             (fun v2 => match v2 with
-                        | VBool b2 => imonad_pure (VBool (b1 || b2))
-                        | _ => imonad_throw (TypeError "")
-                        end)
-       | P2Xor, VBool b1 =>
-           imonad_bind a2
-             (fun v2 => match v2 with
-                        | VBool b2 => imonad_pure (VBool (xorb b1 b2))
-                        | _ => imonad_throw (TypeError "")
-                        end)
+       | P2Add, VInt i1 => imonad_bind a2
+                             (fun v2 => match v2 with
+                                        | VInt i2 => imonad_pure (VInt (i1 + i2))
+                                        | _ => imonad_throw (TypeError "")
+                                        end)
+       | P2Sub, VInt i1 => imonad_bind a2
+                             (fun v2 => match v2 with
+                                        | VInt i2 => imonad_pure (VInt (i1 - i2))
+                                        | _ => imonad_throw (TypeError "")
+                                        end)
+       | P2Mul, VInt i1 => imonad_bind a2
+                             (fun v2 => match v2 with
+                                        | VInt i2 => imonad_pure (VInt (i1 * i2))
+                                        | _ => imonad_throw (TypeError "")
+                                        end)
+       | P2Div, VInt i1 => imonad_bind a2
+                             (fun v2 => match v2 with
+                                        | VInt i2 => imonad_pure (VInt (i1 / i2))
+                                        | _ => imonad_throw (TypeError "")
+                                        end)
+       | P2Rem, VInt i1 => imonad_bind a2
+                             (fun v2 => match v2 with
+                                        | VInt i2 => imonad_pure (VInt (Z.rem i1 i2))
+                                        | _ => imonad_throw (TypeError "")
+                                        end)
+       | P2And, VBool b1 => imonad_bind a2
+                              (fun v2 => match v2 with
+                                         | VBool b2 => imonad_pure (VBool (b1 && b2))
+                                         | _ => imonad_throw (TypeError "")
+                                         end)
+       | P2Or, VBool b1 => imonad_bind a2
+                             (fun v2 => match v2 with
+                                        | VBool b2 => imonad_pure (VBool (b1 || b2))
+                                        | _ => imonad_throw (TypeError "")
+                                        end)
+       | P2Xor, VBool b1 => imonad_bind a2
+                              (fun v2 => match v2 with
+                                         | VBool b2 => imonad_pure (VBool (xorb b1 b2))
+                                         | _ => imonad_throw (TypeError "")
+                                         end)
        | P2Eq, _ => imonad_bind a2 (fun v2 => imonad_pure (VBool (val_eqb v1 v2)))
-       | P2Lt, VInt i1 =>
-           imonad_bind a2
-             (fun v2 => match v2 with
-                        | VInt i2 => imonad_pure (VBool (i1 <? i2))
-                        | _ => imonad_throw (TypeError "")
-                        end)
-       | P2Le, VInt i1 =>
-           imonad_bind a2
-             (fun v2 => match v2 with
-                        | VInt i2 => imonad_pure (VBool (i1 <=? i2))
-                        | _ => imonad_throw (TypeError "")
-                        end)
+       | P2Lt, VInt i1 => imonad_bind a2
+                            (fun v2 => match v2 with
+                                       | VInt i2 => imonad_pure (VBool (i1 <? i2))
+                                       | _ => imonad_throw (TypeError "")
+                                       end)
+       | P2Le, VInt i1 => imonad_bind a2
+                            (fun v2 => match v2 with
+                                       | VInt i2 => imonad_pure (VBool (i1 <=? i2))
+                                       | _ => imonad_throw (TypeError "")
+                                       end)
        | _, _ => imonad_throw (TypeError "")
        end).
 
-Definition interpret_fun (e : expr1) : imonad val :=
-  imonad_map (VFun e) imonad_ask_env.
+Definition interpret_prim2 (p : prim2) (a1 a2 : atom) : imonad val :=
+  interpret_prim2_aux p (interpret_atom a1) (interpret_atom a2).
 
-Definition interpret_fix (e : expr2) : imonad val :=
-  imonad_map (VFix e) imonad_ask_env.
+Definition interpret_fun (t : term1) : imonad val :=
+  imonad_map (fun env => VFun (C1 t env)) imonad_ask_env.
 
-Definition interpret_app (go : expr -> imonad val) (a1 a2 : imonad val) : imonad val :=
+Definition interpret_fix (t : term2) : imonad val :=
+  imonad_map (fun env => VFix (C2 t env)) imonad_ask_env.
+
+Definition interpret_app_aux (go : term -> imonad val) (a1 a2 : imonad val) : imonad val :=
   imonad_bind a1
     (fun v1 =>
        match v1 with
-       | VFun e ve => imonad_bind a2 (fun v2 => imonad_local_env (fun _ => ve) (interpret_expr1_aux go e v2))
-       | VFix e ve => imonad_bind a2 (fun v2 => imonad_local_env (fun _ => ve) (interpret_expr2_aux go e v1 v2))
+       | VFun c => imonad_bind a2 (interpret_clo1_aux go c)
+       | VFix c => imonad_bind a2 (interpret_clo2_aux go c v1)
+       | VKont k => imonad_throw (ControlError "VKont to be implemented")
        | _ => imonad_throw (TypeError "")
        end).
 
-Definition interpret_pair : imonad val -> imonad val -> imonad val :=
-  imonad_lift2 VPair.
+Definition interpret_app (go : term -> imonad val) (a1 a2 : atom) : imonad val :=
+  interpret_app_aux go (interpret_atom a1) (interpret_atom a2).
 
-Definition interpret_fst (a : imonad val) : imonad val :=
-  imonad_bind a
+Definition interpret_pair (a1 a2 : atom) : imonad val :=
+  imonad_lift2 VPair (interpret_atom a1) (interpret_atom a2).
+
+Definition interpret_fst (a : atom) : imonad val :=
+  imonad_bind (interpret_atom a)
     (fun v => match v with
               | VPair v1 _ => imonad_pure v1
               | _ => imonad_throw (TypeError "")
               end).
 
-Definition interpret_snd (a : imonad val) : imonad val :=
-  imonad_bind a
+Definition interpret_snd (a : atom) : imonad val :=
+  imonad_bind (interpret_atom a)
     (fun v => match v with
               | VPair _ v2 => imonad_pure v2
               | _ => imonad_throw (TypeError "")
               end).
 
-Definition interpret_inl : imonad val -> imonad val :=
-  imonad_map VInl.
+Definition interpret_inl (a : atom) : imonad val :=
+  imonad_map VInl (interpret_atom a).
 
-Definition interpret_inr : imonad val -> imonad val :=
-  imonad_map VInr.
+Definition interpret_inr (a : atom) : imonad val :=
+  imonad_map VInr (interpret_atom a).
 
-Definition interpret_case (a : imonad val) (e1 e2 : val -> imonad val) : imonad val :=
-  imonad_bind a
+Definition interpret_case (a : atom) (t1 t2 : val -> imonad val) : imonad val :=
+  imonad_bind (interpret_atom a)
     (fun v => match v with
-              | VInl v' => e1 v'
-              | VInr v' => e2 v'
+              | VInl v' => t1 v'
+              | VInr v' => t2 v'
               | _ => imonad_throw (TypeError "")
               end).
 
-Definition interpret_ref (a : imonad val) : imonad val :=
-  imonad_bind a
+Definition interpret_ref (a : atom) : imonad val :=
+  imonad_bind (interpret_atom a)
     (fun v =>
        imonad_bind imonad_get_state
-         (fun s => match istate_ref v s with
-                   | None => imonad_throw (MemoryError "")
-                   | Some (l, s') => imonad_then (imonad_set_state s') (imonad_pure (VLoc l))
-                   end)).
+         (fun s =>
+            match istate_ref v s with
+            | None => imonad_throw (MemoryError "")
+            | Some (l, s') => imonad_then (imonad_set_state s') (imonad_pure (VLoc l))
+            end)).
 
-Definition interpret_get (a : imonad val) : imonad val :=
-  imonad_bind a
+Definition interpret_get (a : atom) : imonad val :=
+  imonad_bind (interpret_atom a)
     (fun v =>
        match v with
        | VLoc l =>
@@ -174,7 +196,7 @@ Definition interpret_get (a : imonad val) : imonad val :=
        | _ => imonad_throw (TypeError "")
        end).
 
-Definition interpret_set (a1 a2 : imonad val) : imonad val :=
+Definition interpret_set_aux (a1 a2 : imonad val) : imonad val :=
   imonad_bind a1
     (fun v1 =>
        match v1 with
@@ -190,8 +212,11 @@ Definition interpret_set (a1 a2 : imonad val) : imonad val :=
        | _ => imonad_throw (TypeError "")
        end).
 
-Definition interpret_free (a : imonad val) : imonad val :=
-  imonad_bind a
+Definition interpret_set (a1 a2 : atom) : imonad val :=
+  interpret_set_aux (interpret_atom a1) (interpret_atom a2).
+
+Definition interpret_free (a : atom) : imonad val :=
+  imonad_bind (interpret_atom a)
     (fun v =>
        match v with
        | VLoc l =>
@@ -204,54 +229,236 @@ Definition interpret_free (a : imonad val) : imonad val :=
        | _ => imonad_throw (TypeError "")
        end).
 
-Definition interpret_atom (a : atom) : imonad val :=
-  match a with
-  | AVal v => imonad_pure v
-  | AVar x =>
-      imonad_bind imonad_ask_env
-        (fun ve => match venv_lookup x ve with
-                   | None => imonad_throw (NameError "")
-                   | Some v => imonad_pure v
-                   end)
+Fixpoint term_size (t : term) : nat :=
+  match t with
+  | TLet t1 t2 => S (term_size t1 + term1_size t2)
+  | TIf _ t1 t2 => S (Nat.max (term_size t1) (term_size t2))
+  | TShift t' => S (term1_size t')
+  | TReset t' => S (term_size t')
+  | TCase _ t1 t2 => S (Nat.max (term1_size t1) (term1_size t2))
+  | _ => 1
+  end
+with term1_size (t : term1) : nat := let (_, t') := t in term_size t'.
+
+Definition clo1_size (c : clo1) : nat :=
+  let (t, _) := c in term1_size t.
+
+Fixpoint kont_size (k : kont) : nat :=
+  match k with
+  | KNil => 0
+  | KCons c k' => clo1_size c + kont_size k'
   end.
 
-Definition interpret_expr_aux (go : expr -> imonad val) : expr -> imonad val :=
-  fix go' e {struct e} :=
-    match e with
-    | EAtom a => interpret_atom a
-    | ELet e1 e2 => interpret_let (go' e1) (interpret_expr1_aux go' e2)
-    | EIf a e1 e2 => interpret_if (interpret_atom a) (go' e1) (go' e2)
-    | EPrim1 p a => interpret_prim1 p (interpret_atom a)
-    | EPrim2 p a1 a2 => interpret_prim2 p (interpret_atom a1) (interpret_atom a2)
-    | EFun e' => interpret_fun e'
-    | EFix e' => interpret_fix e'
-    | EApp a1 a2 => interpret_app go (interpret_atom a1) (interpret_atom a2)
-    | EPair a1 a2 => interpret_pair (interpret_atom a1) (interpret_atom a2)
-    | EFst a => interpret_fst (interpret_atom a)
-    | ESnd a => interpret_snd (interpret_atom a)
-    | EInl a => interpret_inl (interpret_atom a)
-    | EInr a => interpret_inr (interpret_atom a)
-    | ECase a e1 e2 => interpret_case (interpret_atom a) (interpret_expr1_aux go' e1) (interpret_expr1_aux go' e2)
-    | ERef a => interpret_ref (interpret_atom a)
-    | EGet a => interpret_get (interpret_atom a)
-    | ESet a1 a2 => interpret_set (interpret_atom a1) (interpret_atom a2)
-    | EFree a => interpret_free (interpret_atom a)
-    | EShift _ => imonad_throw (ControlError "shift without enclosing reset")
-    | EReset e' => imonad_throw OutOfFuel
-    | ECont e1 e2 => imonad_throw OutOfFuel
+Local Open Scope nat_scope.
+
+Definition interpret_term1_kont_aux (go : forall (t : term) (k : kont), Acc lt (term_size t + kont_size k) -> imonad val) (t : term1) (v : val) (k : kont) :
+  Acc lt (term1_size t + kont_size k) -> imonad val :=
+  match t with
+  | T1 b t' => fun H_acc =>
+                 let m := go t' k H_acc in
+                 match b with
+                 | BAnon => m
+                 | BVar x => imonad_local_env (ECons x v) m
+                 end
+  end.
+
+Definition interpret_clo1_kont_aux (go : forall (t : term) (k : kont), Acc lt (term_size t + kont_size k) -> imonad val) (c : clo1) (v : val) (k : kont) :
+  Acc lt (clo1_size c + kont_size k) -> imonad val :=
+  match c with C1 t env => fun H_acc => imonad_local_env (fun _ => env) (interpret_term1_kont_aux go t v k H_acc) end.
+
+Definition interpret_kont_aux (go : forall (t : term) (k : kont), Acc lt (term_size t + kont_size k) -> imonad val) (k : kont) (m : imonad val) :
+  Acc lt (kont_size k) -> imonad val :=
+  match k with
+  | KNil => fun _ => m
+  | KCons c k' => fun H_acc => imonad_bind m (fun v => interpret_clo1_kont_aux go c v k' H_acc)
+  end.
+
+Definition interpret_kont_aux' (go : term -> kont -> imonad val) (k : kont) (m : imonad val) : imonad val :=
+  match k with
+  | KNil => m
+  | KCons c k' => imonad_bind m (interpret_clo1_aux (fun t => go t k') c)
+  end.
+
+Definition interpret_term_kont_aux (go : term -> kont -> imonad val) (t : term) (k : kont) : imonad val.
+  refine ((fix go' t k (H_acc : Acc lt (term_size t + kont_size k)) {struct H_acc} : imonad val :=
+             match t return Acc lt (term_size t + kont_size k) -> imonad val with
+             | TAtom a => fun H_acc => interpret_kont_aux go' k (interpret_atom a) _
+             | TLet t1 t2 => fun H_acc => imonad_bind imonad_ask_env (fun env => go' t1 (KCons (C1 t2 env) k) _)
+             | TIf a t1 t2 => fun H_acc => interpret_if a (go' t1 k _) (go' t2 k _)
+             | TPrim1 p a => fun H_acc => interpret_kont_aux go' k (interpret_prim1 p a) _
+             | TPrim2 p a1 a2 => fun H_acc => interpret_kont_aux go' k (interpret_prim2 p a1 a2) _
+             | TFun t' => fun H_acc => interpret_kont_aux go' k (interpret_fun t') _
+             | TFix t' => fun H_acc => interpret_kont_aux go' k (interpret_fix t') _
+             | TApp a1 a2 => fun _ => interpret_app (fun t' => go t' k) a1 a2
+             | TPair a1 a2 => fun H_acc => interpret_kont_aux go' k (interpret_pair a1 a2) _
+             | TFst a => fun H_acc => interpret_kont_aux go' k (interpret_fst a) _
+             | TSnd a => fun H_acc => interpret_kont_aux go' k (interpret_snd a) _
+             | TInl a => fun H_acc => interpret_kont_aux go' k (interpret_inl a) _
+             | TInr a => fun H_acc => interpret_kont_aux go' k (interpret_inr a) _
+             | TCase a t1 t2 => fun H_acc => interpret_case a
+                                               (fun v => interpret_term1_kont_aux go' t1 v k _)
+                                               (fun v => interpret_term1_kont_aux go' t2 v k _)
+             | TShift t' => fun H_acc => interpret_term1_kont_aux go' t' (VKont k) KNil _
+             | TReset t' => fun H_acc => interpret_kont_aux go' k (go' t' KNil _) _
+             | _ => fun _ => imonad_throw OutOfFuel
+             end H_acc) t k (lt_wf _)).
+  - simpl in *. apply (Acc_inv H_acc). lia.
+  - simpl in *. apply (Acc_inv H_acc). lia.
+  - simpl in *. apply (Acc_inv H_acc). lia.
+  - simpl in *. apply (Acc_inv H_acc). lia.
+  - simpl in *. apply (Acc_inv H_acc). lia.
+  - simpl in *. apply (Acc_inv H_acc). lia.
+  - simpl in *. apply (Acc_inv H_acc). lia.
+  - simpl in *. apply (Acc_inv H_acc). lia.
+  - simpl in *. apply (Acc_inv H_acc). lia.
+  - simpl in *. apply (Acc_inv H_acc). lia.
+  - simpl in *. apply (Acc_inv H_acc). lia.
+  - simpl in *. apply (Acc_inv H_acc). lia.
+  - simpl in *. apply (Acc_inv H_acc). lia.
+  - simpl in *. apply (Acc_inv H_acc). lia.
+  - simpl in *. apply (Acc_inv H_acc). lia.
+  - simpl in *. apply (Acc_inv H_acc). lia.
+  - simpl in *. apply (Acc_inv H_acc). lia.
+  - simpl in *. apply (Acc_inv H_acc). lia.
+Defined.
+
+Local Close Scope nat_scope.
+
+Definition interpret_term_kont_bot (_ : term) (_ : kont) : imonad val :=
+  imonad_throw OutOfFuel.
+
+Fixpoint interpret_term_kont (fuel : nat) (t : term) (k : kont) : imonad val :=
+  match fuel with
+  | O => interpret_term_kont_bot
+  | S fuel' => interpret_term_kont_aux (interpret_term_kont fuel')
+  end t k.
+
+(*
+Definition interpret_term_cont_aux (go : term -> imonad val) (go_cont : clo1 -> term -> imonad val) : clo1 -> term -> imonad val :=
+  fix go_cont' k t {struct t} :=
+    match t with
+    | TAtom a => imonad_bind (interpret_atom a) (interpret_clo1_aux go k)
+    | TLet t1 t2 => imonad_bind imonad_ask_env (fun env => go_cont' (C1 (compose t2 k) env) t1)
+    | TIf a t1 t2 => interpret_if a (go_cont' k t1) (go_cont' k t2)
+    | TPrim1 p a => imonad_bind (interpret_prim1 p a) (interpret_clo1_aux go k)
+    | TPrim2 p a1 a2 => imonad_bind (interpret_prim2 p a1 a2) (interpret_clo1_aux go k)
+    | TFun t' => imonad_bind (interpret_fun t') (interpret_clo1_aux go k)
+    | TFix t' => imonad_bind (interpret_fix t') (interpret_clo1_aux go k)
+    | TApp a1 a2 => interpret_app (go_cont k) a1 a2
+    | TPair a1 a2 => imonad_bind (interpret_pair a1 a2) (interpret_clo1_aux go k)
+    | TFst a => imonad_bind (interpret_fst a) (interpret_clo1_aux go k)
+    | TSnd a => imonad_bind (interpret_snd a) (interpret_clo1_aux go k)
+    | TInl a => imonad_bind (interpret_inl a) (interpret_clo1_aux go k)
+    | TInr a => imonad_bind (interpret_inr a) (interpret_clo1_aux go k)
+    | TCase a t1 t2 => interpret_case a (interpret_term1_aux (go_cont' k) t1) (interpret_term1_aux (go_cont' k) t2)
+    | TShift t' => interpret_term1_aux (go_cont' identity) t' (VFun k)
+    | TReset t' => imonad_bind (go_cont' identity t') (interpret_clo1_aux go k)
+    | TCont t' k' => imonad_bind (go_cont' k'  t') (interpret_clo1_aux go k)
+    | _ => imonad_throw OutOfFuel
+    end.
+*)
+
+Definition interpret_app_aux' (go : term -> imonad val) (go_cont : term -> kont -> imonad val) (a1 a2 : imonad val) : imonad val :=
+  imonad_bind a1
+    (fun v1 =>
+       match v1 with
+       | VFun c => imonad_bind a2 (interpret_clo1_aux go c)
+       | VFix c => imonad_bind a2 (interpret_clo2_aux go c v1)
+       | VKont k => interpret_kont_aux' go_cont k a2
+       | _ => imonad_throw (TypeError "")
+       end).
+
+Definition interpret_app' (go : term -> imonad val) (go_cont : term -> kont -> imonad val) (a1 a2 : atom) : imonad val :=
+  interpret_app_aux' go go_cont (interpret_atom a1) (interpret_atom a2).
+
+Definition interpret_term_aux (go : term -> imonad val) (go_kont : term -> kont -> imonad val) : term -> imonad val :=
+  fix go' t {struct t} :=
+    match t with
+    | TAtom a => interpret_atom a
+    | TLet t1 t2 => imonad_bind (go' t1) (interpret_term1_aux go' t2)
+    | TIf a t1 t2 => interpret_if a (go' t1) (go' t2)
+    | TPrim1 p a => interpret_prim1 p a
+    | TPrim2 p a1 a2 => interpret_prim2 p a1 a2
+    | TFun t' => interpret_fun t'
+    | TFix t' => interpret_fix t'
+    | TApp a1 a2 => interpret_app' go go_kont a1 a2
+    | TPair a1 a2 => interpret_pair a1 a2
+    | TFst a => interpret_fst a
+    | TSnd a => interpret_snd a
+    | TInl a => interpret_inl a
+    | TInr a => interpret_inr a
+    | TCase a t1 t2 => interpret_case a (interpret_term1_aux go' t1) (interpret_term1_aux go' t2)
+    | TRef a => interpret_ref a
+    | TGet a => interpret_get a
+    | TSet a1 a2 => interpret_set a1 a2
+    | TFree a => interpret_free a
+    | TShift _ => imonad_throw (ControlError "shift without enclosing reset")
+    | TReset t' => go_kont t' KNil
+    (*| TCont t' k => interpret_term_kont_aux go_kont t' k*)
+    | TCont _ _ => imonad_throw (ControlError "TCont not supported!")
     end.
 
-Fixpoint interpret_expr (fuel : nat) : expr -> imonad val :=
-  interpret_expr_aux (match fuel with
-                      | O => fun _ => imonad_throw OutOfFuel
-                      | S fuel' => interpret_expr fuel'
-                      end).
+Definition interpret_term_bot (_ : term) : imonad val :=
+  imonad_throw OutOfFuel.
 
-Definition run (fuel : nat) (e : expr) : (ierror + val) * istate :=
-  interpret_expr fuel e VENil istate_empty.
+Fixpoint interpret_term (fuel : nat) (t : term) : imonad val :=
+  match fuel with
+  | O => interpret_term_aux interpret_term_bot interpret_term_kont_bot
+  | S fuel' => interpret_term_aux (interpret_term fuel') (interpret_term_kont fuel)
+  end t.
 
-Definition eval (fuel : nat) (e : expr) : ierror + val :=
+Definition run (fuel : nat) (e : term) : (ierror + val) * istate :=
+  interpret_term fuel e ENil istate_empty.
+
+Definition eval (fuel : nat) (e : term) : ierror + val :=
   fst (run fuel e).
 
-Definition exec (fuel : nat) (e : expr) : istate :=
+Definition exec (fuel : nat) (e : term) : istate :=
   snd (run fuel e).
+
+Import Coerce.
+Example f := TReset (TLet
+                       (TPrim2 P2Mul (VInt 6) (VInt 9))
+                       (T1 (Var "x")
+                          (TLet
+                             (TShift (T1 (Var "k") (Var "k")))
+                             (T1 (Var "y") (TPrim2 P2Add (Var "x") (Var "y")))))).
+Example fx := TLet f (T1 (Var "f") (TApp (Var "f") (VInt 10))).
+Compute (eval 1 fx).
+
+Example append :=
+  TFix
+    (T2 (Var "f")
+       (T1 (Var "xs")
+          (TCase (Var "xs")
+             (T1 BAnon (TShift (T1 (Var "k") (Var "k"))))
+             (T1 (Var "p")
+                (TLet
+                   (TFst (Var "p"))
+                   (T1 (Var "x")
+                      (TLet
+                         (TSnd (Var "p"))
+                         (T1 (Var "xs'")
+                            (TLet
+                               (TApp (Var "f") (Var "xs'"))
+                               (T1 (Var "r")
+                                  (TLet
+                                     (TPair (Var "x") (Var "r"))
+                                     (T1 (Var "r'") (TInr (Var "r'")))))))))))))).
+
+Fixpoint encode (xs : list Z) : val :=
+  match xs with
+  | nil => VInl VUnit
+  | cons x xs' => VInr (VPair (VInt x) (encode xs'))
+  end.
+
+Example wrap_append v1 :=
+  TReset (TLet append (T1 (Var "append") (TApp (Var "append") v1))).
+Example use_append v1 v2 :=
+  TLet (wrap_append v1)
+    (T1 (Var "f") (TApp (Var "f") v2)).
+
+Example append1 := use_append (encode nil) (encode (1 :: nil)).
+Example append2 := use_append (encode (1 :: 2 :: 3 :: 4 :: nil)) (encode (4 :: 5 :: 6 :: 7 :: nil)).
+
+Compute (eval 2 (wrap_append (encode (nil)))).
