shift-reset/core/env.v
@@ -1,0 +1,8 @@
+From shift_reset.core Require Import var syntax.
+
+Definition env_lookup (x : var) : env -> option val :=
+  fix go env :=
+    match env with
+    | ENil => None
+    | ECons x' v env' => if var_eq_dec x x' then Some v else go env'
+    end.
