shift-reset/interpreter/imonad.v
@@ -2,13 +2,13 @@ From shift_reset.lib Require Import sum.
 From shift_reset.core Require Import syntax.
 From shift_reset.interpreter Require Import istate ierror.
 
-Definition imonad (A : Type) : Type := venv -> istate -> (ierror + A) * istate.
+Definition imonad (A : Type) : Type := env -> istate -> (ierror + A) * istate.
 
-Definition imonad_ask_env : imonad venv :=
-  fun ve s => (inr ve, s).
+Definition imonad_ask_env : imonad env :=
+  fun env s => (inr env, s).
 
-Definition imonad_local_env {A} (f : venv -> venv) (m : imonad A) : imonad A :=
-  fun ve s => m (f ve) s.
+Definition imonad_local_env {A} (f : env -> env) (m : imonad A) : imonad A :=
+  fun env s => m (f env) s.
 
 Definition imonad_get_state : imonad istate :=
   fun _ s => (inr s, s).
@@ -23,8 +23,8 @@ Definition imonad_throw {A} (e : ierror) : imonad A :=
   fun _ s => (inl e, s).
 
 Definition imonad_map {A B} (f : A -> B) (m : imonad A) :=
-  fun ve s =>
-    let (r, s) := m ve s in
+  fun env s =>
+    let (r, s) := m env s in
     match r with
     | inl e => (inl e, s)
     | inr x => (inr (f x), s)
@@ -34,12 +34,12 @@ Definition imonad_pure {A} (x : A) : imonad A :=
   fun _ s => (inr x, s).
 
 Definition imonad_lift2 {A B C} (f : A -> B -> C) (m1 : imonad A) (m2 : imonad B) : imonad C :=
-  fun ve s =>
-    let (r, s) := m1 ve s in
+  fun env s =>
+    let (r, s) := m1 env s in
     match r with
     | inl e => (inl e, s)
     | inr x =>
-        let (r, s) := m2 ve s in
+        let (r, s) := m2 env s in
         match r with
         | inl e => (inl e, s)
         | inr y => (inr (f x y), s)
@@ -47,17 +47,17 @@ Definition imonad_lift2 {A B C} (f : A -> B -> C) (m1 : imonad A) (m2 : imonad B
     end.
 
 Definition imonad_bind {A B} (m : imonad A) (f : A -> imonad B) : imonad B :=
-  fun ve s =>
-    let (r, s) := m ve s in
+  fun env s =>
+    let (r, s) := m env s in
     match r with
     | inl e => (inl e, s)
-    | inr x => f x ve s
+    | inr x => f x env s
     end.
 
 Definition imonad_then {A B} (m1 : imonad A) (m2 : imonad B) : imonad B :=
-  fun ve s =>
-    let (r, s) := m1 ve s in
+  fun env s =>
+    let (r, s) := m1 env s in
     match r with
     | inl e => (inl e, s)
-    | inr _ => m2 ve s
+    | inr _ => m2 env s
     end.
